proofs/lean/SpecRest/Translate.lean
@@ -41,6 +41,7 @@ def translate : Expr → SmtTerm
   | .enumAccess en memberName => .enumElemConst en memberName
   | .member elem relName     => .inDom relName (translate elem)
   | .forallEnum var en body  => .forallEnum var en (translate body)
+  | .forallRel  var rel body => .forallRel var rel (translate body)
   | .prime e                  => translate e
   | .pre   e                  => translate e
   | .cardRel relName          => .cardRel relName
